---
aliases:
  - UARM
  - Moto Rettilineo Uniformemente Accelerato
---
${ a(t) = a_{0} = const = \frac{dv}{dt} }$
${ \underbrace{ \int^{v_{2}}_{v_{1}}dv }_{ \Delta v=v_{2}-v_{1} } = \underbrace{ \int^{t_{2}}_{t_{1}}a_{0}dt }_{ a_{0}(t_{2}-t_{1}) } }$

${ \boxed{ \underset{ v }{ v_{2} }-\underset{ v_{i} }{ v_{1} } = a_{0}(\underset{ t }{ t_{2} }-\underset{ t_{i} }{ t_{1} }) } \longrightarrow \boxed{v = a_{0}t}  }$

${ v = \frac{dx}{dt} \longrightarrow dx = Vdt = a_{0}tdt }$
${ v = \frac{dx}{dt} \longrightarrow \underbrace{ \int^{x_{2}}_{x_{1}} dx }_{  } = Vdt = \int^{t_{2}}_{t_{1}} a_{0}tdt }$
${ \Delta x = a_{0} \int^{t_{2}}_{t_{1}}tdt }$

${ x_{2}-x_{1} = \frac{a_{0}1}{2} [t_{2}^{2}-t_{1}^{2}] }$

${ \frac{1}{2}vt = \frac{1}{2}a_{0}t^{2} }$

${ v=a_{0}(t_{2}-t_{1})+ v_{0} }$

---

kinematic law for ${ t_{0} = 0 }$

1. ${ x = x_{0} \pm v_{0}(t-t_{0}) + \frac{1}{2} a_{0}(t^{2}-t_{0}^{2}) }$
2. ${ v=v_{0}\pm a_{0}(t-t_{0}) }$
3. ![[#^thingy]]

---

${ v[x(t)] }$

${ a=\frac{dv}{dt} = \frac{d}{dt}[v(x(t))] = \frac{dv}{dx} \frac{dx}{dt} = v \frac{dv}{dx} }$
${ a = v \frac{dv}{dx} \longrightarrow \int^{x_{2}}_{x_{1}}a dx = \int^{v_{2}}_{v_{1}}v dv }$

${ \Downarrow }$
${ \boxed{ \int^{x_{2}}_{x_{1}}a dx = \frac{1}{2} [ v_{2}^{2} - v_{1}^{2}] } }$

${ \int^{x_{2}}_{x_{1}} a_{0}dx = \frac{1}{2} (v_{2}^{2} - v_{1}^{2}) }$
${ a_{0}(x_{2}-x_{1}) = \frac{1}{2} (v_{2}^{2}-v_{1}^{2}) }$

${ v^{2} = v_{0}^{2} \pm 2 a_{0} (x_{2}-x_{1}) }$ ^thingy

---

${ x = x_{0}+v_{0}t \pm \frac{1}{2}|g|t^{2} }$
${ v = v_{0} \pm |g| t }$
${ v^{2} = v_{0}^{2} \pm 2|g| t }$

${ \Delta x = x_{2}-x_{1} < 0 }$
${ |v_{2}| > |v_{1}| }$

${ \Delta x = x_{2}-x_{1} < 0 }$
${ \Delta v = v_{2}-v_{1}<0 }$

${ \Delta x = x_{2}-x_{1} > 0 }$
${ \Delta v = v_{2}-v_{1} >0 }$